prove the equivalence between two versions of CPA LR and b.

theories/crypto/PKE.ec
@@ -6,8 +6,7 @@
  * Distributed under the terms of the CeCILL-B-V1 license
  * -------------------------------------------------------------------- *)
 
-require import Bool Core Int List.
-require import DBool.
+require import AllCore List Distr DBool LorR.
 
 type pkey.
 type skey.
@@ -42,6 +41,62 @@ module CPA (S:Scheme, A:Adversary) = {
   }
 }.
 
+module CPA_L (S:Scheme, A:Adversary) = {
+  proc main() : bool = {
+    var pk : pkey;
+    var sk : skey;
+    var m0, m1 : plaintext;
+    var c : ciphertext;
+    var b' : bool;
+
+    (pk, sk) = S.kg();
+    (m0, m1) = A.choose(pk);
+    c        = S.enc(pk, m0);
+    b'       = A.guess(c);
+    return b';
+  }
+}.
+
+module CPA_R (S:Scheme, A:Adversary) = {
+  proc main() : bool = {
+    var pk : pkey;
+    var sk : skey;
+    var m0, m1 : plaintext;
+    var c : ciphertext;
+    var b' : bool;
+
+    (pk, sk) = S.kg();
+    (m0, m1) = A.choose(pk);
+    c        = S.enc(pk, m1);
+    b'       = A.guess(c);
+    return b';
+  }
+}.
+
+section.
+
+  declare module S:Scheme.
+  declare module A:Adversary{S}.
+
+  lemma pr_CPA_LR &m: 
+    islossless S.kg => islossless S.enc =>
+    islossless A.choose => islossless A.guess => 
+    `| Pr[CPA_L(S,A).main () @ &m : res] - Pr[CPA_R(S,A).main () @ &m : res] | =
+     2%r * `| Pr[CPA(S,A).main() @ &m : res] - 1%r/2%r |.
+  proof.
+    move => kg_ll enc_ll choose_ll guess_ll.
+    have -> : Pr[CPA(S, A).main() @ &m : res] = 
+              Pr[RandomLR(CPA_R(S,A), CPA_L(S,A)).main() @ &m : res].
+    + byequiv (_ : ={glob S, glob A} ==> ={res})=> //.
+      proc.      
+      swap{1} 3-2; seq 1 1 : (={glob S, glob A, b}); first by rnd.
+      if{2}; inline *; wp; do 4! call (_: true); auto => /> /#.
+    rewrite -(pr_AdvLR_AdvRndLR (CPA_R(S,A)) (CPA_L(S,A)) &m) 2:/#.
+    byphoare => //; proc.
+    by call guess_ll; call enc_ll; call choose_ll; call kg_ll.
+  qed.
+
+end section.
 
 (*
 ** Based on lists. Several versions can be given as in RandOrcl.
