theories/crypto/LorR.ec
@@ -1,0 +1,70 @@
+require import AllCore Distr DBool.
+
+module type A = {
+  proc main() : bool
+}.
+
+module RandomLR(L:A) (R:A) = {
+  proc main () = { 
+    var b,r : bool;
+    b <${0,1};
+    if (b)  r <@ L.main();
+    else r <@ R.main ();
+    return (b = r);
+  }
+}.
+
+section.
+
+  declare module L:A.
+  declare module R:A.
+
+  local module Aux = {
+    var b,r : bool
+    proc main () = { 
+      b <${0,1};
+      if (b)  r <@ L.main();
+      else r <@ R.main ();
+      return (b = r);
+    }
+  }.
+
+  lemma pr_AdvLR_AdvRndLR &m: 
+     Pr[R.main() @ &m : true] = 1%r =>
+     `| Pr[L.main () @ &m : res] - Pr[R.main () @ &m : res] | =
+     2%r * `| Pr[RandomLR(L, R).main() @ &m : res] - 1%r/2%r |.
+  proof.
+    move => Hll.
+    have -> : Pr[RandomLR(L, R).main() @ &m : res] = Pr[Aux.main() @ &m : res].
+    + by byequiv => //; proc; sim=> /#.
+    have -> : Pr[Aux.main() @ &m : res] = 
+              Pr[Aux.main() @ &m : res /\ Aux.b] +  
+              Pr[Aux.main() @ &m : res /\ !Aux.b].
+    + by rewrite Pr [mu_split Aux.b].
+    have -> : Pr[Aux.main() @ &m : res /\ Aux.b] = 1%r/2%r * Pr[L.main () @ &m : res].
+    + byphoare (_: (glob L) = (glob L){m} ==> res /\ Aux.b) => //.
+      proc; pose p := Pr[L.main() @ &m : res]. (* FIXME assert false without the pose *)
+      seq 1 : (Aux.b = true) (1%r/2%r) p  _ 0%r (glob L = (glob L){m}); 1:by auto.
+      + by rnd (pred1 true); skip => />; rewrite dbool1E.
+      + if; last by (conseq (_: false ==> _); 1:by smt()); auto.
+        conseq (_ : _ ==> Aux.r) => //; 1:by smt().
+        call (_: glob L = (glob L){m} ==> res); last by auto.
+        by bypr=> &m0 hm0; rewrite /p; byequiv=> //; proc (true).
+      + by (conseq (_: _ ==> false); 1:smt()); auto.
+      smt().
+    have -> : Pr[Aux.main() @ &m : res /\ !Aux.b] = 1%r/2%r * Pr[R.main () @ &m : !res].
+    + byphoare (_: (glob R) = (glob R){m} ==> res /\ !Aux.b) => //.
+      proc; pose p := Pr[R.main() @ &m : !res]. 
+      seq 1 : (Aux.b = false) (1%r/2%r) p  _ 0%r (glob R = (glob R){m}); 1:by auto.
+      + by rnd (pred1 false); skip => />; rewrite dbool1E.
+      + if; first by (conseq (_: false ==> _); 1:by smt()); auto.
+        conseq (_ : _ ==> !Aux.r) => //; 1:by smt().
+        call (_: glob R = (glob R){m} ==> !res); last by auto.
+        by bypr=> &m0 hm0; rewrite /p; byequiv=> //; proc (true).
+      + by (conseq (_: _ ==> false); 1:smt()); auto.
+      smt().
+    rewrite Pr [mu_not] Hll /#.
+  qed.
+
+end section.
+
